\section*{Question 3}

\noindent
\emph{Sans avoir recours aux tables de vérité (utilisez le Théorème 1), montrez que les deux propositions
suivantes sont équivalentes}
\[\neg p \vee  (r \Rightarrow (\neg q)) \equiv \neg p \vee \neg q \vee \neg r\]

\begin{align*}
	\neg p \vee (r \Rightarrow (\neg q)) & \equiv \neg p \vee \neg(\neg(r \Rightarrow (\neg q)) \\
	                                     & \equiv \neg p \vee \neg(r \wedge \neg(\neg q))       \\
	                                     & \equiv \neg p \vee \neg r \vee \neg q
\end{align*}